Main.lean
@@ -12,12 +12,30 @@ def allDecs: (M: Machine l s) → HaltM M Unit := λ M ↦ do
   noHaltDec M
   (looperDec 20 M)
 
-#eval (Busybeaver.BBCompute (l:=1) (s:=1) allDecs (λ lab sym ↦ if lab = default ∧ sym = default then
-Stmt.next 1 .right 1 else .halt)).undec
+/- #eval .undec -/
 
+def compute (l s: ℕ): Busybeaver.BBResult l s :=
+  let res0 := Task.spawn (λ _ ↦ (Busybeaver.BBCompute allDecs (Busybeaver.BBCompute.m0RB l s)))
+  let res1 := Task.spawn (λ _ ↦ (Busybeaver.BBCompute allDecs (Busybeaver.BBCompute.m1RB l s)))
+  Busybeaver.BBResult.join res0.get res1.get
 /- def all22 := (Finset.univ (α:=TM22)).filter (λ M ↦ M default default = .next 1 .right 1) -/
 
-/- set_option compiler.extract_closed false -/
+axiom task_correct {α: Type} {f: Unit → α}: (Task.spawn f |>.get) = f ()
+
+set_option compiler.extract_closed false
+def main: IO Unit := do
+  IO.println "Starting computation"
+  let comp := compute 1 3
+  if hcomp: comp.undec = ∅ then
+    have _: comp.val = Busybeaver 1 3 := by {
+      simp [comp] at *
+      simp [compute, task_correct]
+      exact Eq.symm (Busybeaver.BBCompute.correct_complete hcomp)
+    }
+    IO.println s!"Busybeaver = {comp.val}"
+  else
+    IO.println s!"#Undecided: {comp.undec.card}"
+
 /- def main : IO Unit := do -/
 /-   IO.println "Compute initial set"; -/
 /-   let init := all22; -/
